[ML-KEM] F* extraction for polynomial

libcrux-iot/ml-kem/hax.py
@@ -72,7 +72,7 @@ class extractAction(argparse.Action):
             # "+libcrux_iot_ml_kem::spec::*",
             # "+libcrux_iot_ml_kem::vector::**",
             "+libcrux_iot_ml_kem::vector::**",
-            # "+libcrux_iot_ml_kem::polynomial::**"
+            "+libcrux_iot_ml_kem::polynomial::**"
             # "+libcrux_iot_ml_kem::vector::portable::arithmetic::**",
             # "+libcrux_iot_ml_kem::vector::portable::ntt::**",
             # "+libcrux_iot_ml_kem::vector::portable::sampling::**",
